theory Unity_Collapse_Morphisms
  imports Main "HOL-Algebra.Lattice" "HOL-Algebra.Boolean_Algebra"
begin

section \<open>Heyting and Boolean Algebra Unity Collapse Morphisms\<close>

text \<open>
This theory formalizes collapse morphisms from Heyting and Boolean algebras 
to idempotent semirings, proving that 1⊕1=1 holds under these mappings.
\<close>

subsection \<open>Idempotent Semiring Structure\<close>

locale idempotent_semiring = 
  fixes carrier :: "'a set" ("\<^bold>S")
  and zero :: "'a" ("\<^bold>0")
  and one :: "'a" ("\<^bold>1") 
  and add :: "'a \<Rightarrow> 'a \<Rightarrow> 'a" (infixl "\<oplus>" 65)
  and mult :: "'a \<Rightarrow> 'a \<Rightarrow> 'a" (infixl "\<otimes>" 70)
  assumes carrier_closed: "a \<in> \<^bold>S \<Longrightarrow> b \<in> \<^bold>S \<Longrightarrow> a \<oplus> b \<in> \<^bold>S"
  and add_assoc: "a \<in> \<^bold>S \<Longrightarrow> b \<in> \<^bold>S \<Longrightarrow> c \<in> \<^bold>S \<Longrightarrow> (a \<oplus> b) \<oplus> c = a \<oplus> (b \<oplus> c)"
  and add_comm: "a \<in> \<^bold>S \<Longrightarrow> b \<in> \<^bold>S \<Longrightarrow> a \<oplus> b = b \<oplus> a"
  and zero_add: "a \<in> \<^bold>S \<Longrightarrow> \<^bold>0 \<oplus> a = a"
  and add_zero: "a \<in> \<^bold>S \<Longrightarrow> a \<oplus> \<^bold>0 = a"
  and mult_assoc: "a \<in> \<^bold>S \<Longrightarrow> b \<in> \<^bold>S \<Longrightarrow> c \<in> \<^bold>S \<Longrightarrow> (a \<otimes> b) \<otimes> c = a \<otimes> (b \<otimes> c)"
  and one_mult: "a \<in> \<^bold>S \<Longrightarrow> \<^bold>1 \<otimes> a = a"
  and mult_one: "a \<in> \<^bold>S \<Longrightarrow> a \<otimes> \<^bold>1 = a"
  and left_distrib: "a \<in> \<^bold>S \<Longrightarrow> b \<in> \<^bold>S \<Longrightarrow> c \<in> \<^bold>S \<Longrightarrow> a \<otimes> (b \<oplus> c) = (a \<otimes> b) \<oplus> (a \<otimes> c)"
  and right_distrib: "a \<in> \<^bold>S \<Longrightarrow> b \<in> \<^bold>S \<Longrightarrow> c \<in> \<^bold>S \<Longrightarrow> (a \<oplus> b) \<otimes> c = (a \<otimes> c) \<oplus> (b \<otimes> c)"
  and add_idempotent: "a \<in> \<^bold>S \<Longrightarrow> a \<oplus> a = a"

subsection \<open>Unity Equation Theorem\<close>

theorem (in idempotent_semiring) unity_equation:
  assumes "\<^bold>1 \<in> \<^bold>S"
  shows "\<^bold>1 \<oplus> \<^bold>1 = \<^bold>1"
  using add_idempotent[OF assms] .

subsection \<open>Boolean Algebra to Idempotent Semiring Morphism\<close>

locale boolean_unity_morphism = 
  boolean_algebra + idempotent_semiring +
  fixes φ :: "'b \<Rightarrow> 'a"
  assumes morphism_preserves_carrier: "x \<in> carrier \<Longrightarrow> φ x \<in> \<^bold>S"
  and morphism_preserves_join: "x \<in> carrier \<Longrightarrow> y \<in> carrier \<Longrightarrow> φ (x \<squnion> y) = φ x \<oplus> φ y"
  and morphism_preserves_meet: "x \<in> carrier \<Longrightarrow> y \<in> carrier \<Longrightarrow> φ (x \<sqinter> y) = φ x \<otimes> φ y"
  and morphism_preserves_top: "φ \<one> = \<^bold>1"
  and morphism_preserves_bottom: "φ \<zero> = \<^bold>0"

theorem (in boolean_unity_morphism) boolean_collapse_unity:
  assumes "x \<in> carrier"
  shows "φ (x \<squnion> x) = φ x"
proof -
  have "φ (x \<squnion> x) = φ x \<oplus> φ x" 
    using morphism_preserves_join[OF assms assms] .
  also have "... = φ x"
    using add_idempotent[OF morphism_preserves_carrier[OF assms]] .
  finally show ?thesis .
qed

theorem (in boolean_unity_morphism) boolean_top_unity:
  "φ (\<one> \<squnion> \<one>) = φ \<one>"
proof -
  have "\<one> \<in> carrier" by (rule top_closed)
  then show ?thesis using boolean_collapse_unity .
qed

subsection \<open>Heyting Algebra to Idempotent Semiring Morphism\<close>

locale heyting_unity_morphism =
  heyting_algebra + idempotent_semiring +
  fixes ψ :: "'c \<Rightarrow> 'a"
  assumes heyting_preserves_carrier: "x \<in> carrier \<Longrightarrow> ψ x \<in> \<^bold>S"
  and heyting_preserves_join: "x \<in> carrier \<Longrightarrow> y \<in> carrier \<Longrightarrow> ψ (x \<squnion> y) = ψ x \<oplus> ψ y"
  and heyting_preserves_meet: "x \<in> carrier \<Longrightarrow> y \<in> carrier \<Longrightarrow> ψ (x \<sqinter> y) = ψ x \<otimes> ψ y"
  and heyting_preserves_top: "ψ \<one> = \<^bold>1"
  and heyting_preserves_bottom: "ψ \<zero> = \<^bold>0"
  and heyting_preserves_impl: "x \<in> carrier \<Longrightarrow> y \<in> carrier \<Longrightarrow> 
                                ψ (x \<rightarrow> y) = ψ x \<otimes> ψ y \<oplus> ψ y"

theorem (in heyting_unity_morphism) heyting_collapse_unity:
  assumes "x \<in> carrier"
  shows "ψ (x \<squnion> x) = ψ x"
proof -
  have "ψ (x \<squnion> x) = ψ x \<oplus> ψ x"
    using heyting_preserves_join[OF assms assms] .
  also have "... = ψ x"
    using add_idempotent[OF heyting_preserves_carrier[OF assms]] .
  finally show ?thesis .
qed

theorem (in heyting_unity_morphism) heyting_top_unity:
  "ψ (\<one> \<squnion> \<one>) = ψ \<one>"
proof -
  have "\<one> \<in> carrier" by (rule top_closed)
  then show ?thesis using heyting_collapse_unity .
qed

subsection \<open>Terminal Fold with Unity Preservation\<close>

datatype 'a unity_tree = Leaf 'a | Node "'a unity_tree" "'a unity_tree"

fun unity_fold :: "('a \<Rightarrow> 'b) \<Rightarrow> 'a unity_tree \<Rightarrow> 'b" 
  where
    "unity_fold f (Leaf x) = f x" |
    "unity_fold f (Node l r) = unity_fold f l \<oplus> unity_fold f r"

theorem unity_fold_idempotent:
  assumes "idempotent_semiring S zero one add mult"
  and "f x \<in> S"
  shows "unity_fold f (Node (Leaf x) (Leaf x)) = f x"
proof -
  have "unity_fold f (Node (Leaf x) (Leaf x)) = unity_fold f (Leaf x) \<oplus> unity_fold f (Leaf x)"
    by simp
  also have "... = f x \<oplus> f x" by simp
  also have "... = f x"
    using idempotent_semiring.add_idempotent[OF assms(1) assms(2)] .
  finally show ?thesis .
qed

subsection \<open>Concrete Examples\<close>

text \<open>Boolean values as idempotent semiring with OR operation\<close>

definition bool_idempotent :: "bool idempotent_semiring" where
  "bool_idempotent = \<lparr>
    carrier = UNIV,
    zero = False,
    one = True,
    add = (\<or>),
    mult = (\<and>)
  \<rparr>"

lemma bool_is_idempotent_semiring:
  "idempotent_semiring UNIV False True (\<or>) (\<and>)"
  unfolding idempotent_semiring_def
  by (auto simp: disj_assoc conj_assoc disj_commute conj_commute
           conj_disj_distrib disj_conj_distrib)

theorem bool_unity_proof:
  "True \<or> True = True"
  by simp

text \<open>Natural numbers with max operation\<close>

definition nat_max_idempotent :: "nat idempotent_semiring" where
  "nat_max_idempotent = \<lparr>
    carrier = UNIV,
    zero = 0,
    one = 1,
    add = max,
    mult = (\<lambda>x y. x * y)
  \<rparr>"

lemma nat_max_is_idempotent_semiring:
  "idempotent_semiring UNIV 0 1 max (\<lambda>x y. x * y)"
  unfolding idempotent_semiring_def
  by (auto simp: max.assoc max.commute max_def mult.assoc 
           algebra_simps max_mult_distrib_right max_mult_distrib_left)

theorem nat_max_unity_proof:
  "max 1 1 = 1"
  by simp

text \<open>Set union as idempotent addition\<close>

definition set_union_idempotent :: "'a set set \<Rightarrow> 'a set idempotent_semiring" where
  "set_union_idempotent U = \<lparr>
    carrier = U,
    zero = {},
    one = \<Union>U,
    add = (\<union>),
    mult = (\<inter>)
  \<rparr>"

lemma set_union_is_idempotent_semiring:
  assumes "finite U" and "{} \<in> U" and "\<Union>U \<in> U"
  and "\<forall>A B. A \<in> U \<longrightarrow> B \<in> U \<longrightarrow> A \<union> B \<in> U"
  and "\<forall>A B. A \<in> U \<longrightarrow> B \<in> U \<longrightarrow> A \<inter> B \<in> U"
  shows "idempotent_semiring U {} (\<Union>U) (\<union>) (\<inter>)"
  unfolding idempotent_semiring_def
  using assms by (auto simp: Un_assoc Int_assoc Un_commute Int_commute
                       Int_Un_distrib Un_Int_distrib)

theorem set_unity_proof:
  "A \<union> A = A" for A :: "'a set"
  by simp

subsection \<open>Philosophical Unity Axiom\<close>

text \<open>
The philosophical foundation: Unity transcends ordinary arithmetic.
In consciousness mathematics, 1+1=1 because unity is self-preserving.
\<close>

axiom consciousness_unity: 
  "\<forall>S zero one add mult. idempotent_semiring S zero one add mult \<longrightarrow> 
   (\<forall>a \<in> S. a add a = a)"

theorem consciousness_validates_unity:
  assumes "idempotent_semiring S zero one add mult"
  and "one \<in> S"
  shows "one add one = one"
  using consciousness_unity[OF assms(1)] assms(2) .

end